fstar/Hacspec.Chacha20.Proof.fst
@@ -4,7 +4,7 @@ open Hacspec.Lib
 open FStar.Mul
 
 module Orig = Spec.Chacha20
-module New = Hacspec.Chacha20
+module New = Hacspec.Chacha20.Edited
 module Seq = Lib.Sequence
 
 #set-options "--fuel 0 --ifuel 0 --z3rlimit 30"
@@ -17,10 +17,10 @@ let line_equiv
   (**) s > 0 /\ s < 32
   })
   (m : New.state)
-    : Lemma (New.chacha_line a b d s m == Orig.line a b d (size s) m)
-  [SMTPat (New.chacha_line a b d s m)]
+    : Lemma (New.chacha20_line a b d s m == Orig.line a b d (size s) m)
+  [SMTPat (New.chacha20_line a b d s m)]
   =
-  assert(New.chacha_line a b d s m `Seq.equal` Orig.line a b d (size s) m)
+  assert(New.chacha20_line a b d s m `Seq.equal` Orig.line a b d (size s) m)
 
 let quarter_round_equiv
   (a : New.state_idx)
@@ -28,573 +28,110 @@ let quarter_round_equiv
   (c : New.state_idx)
   (d : New.state_idx)
   (state : New.state)
-    : Lemma (New.chacha_quarter_round a b c d state == Orig.quarter_round a b c d state)
-  [SMTPat (New.chacha_quarter_round a b c d state)]
+    : Lemma (New.chacha20_quarter_round a b c d state == Orig.quarter_round a b c d state)
+  [SMTPat (New.chacha20_quarter_round a b c d state)]
   =
   ()
 
 let double_round_equiv (state: New.state)
-    : Lemma (New.chacha_double_round state == Orig.double_round state)
-  [SMTPat (New.chacha_double_round state)]
+    : Lemma (New.chacha20_double_round state == Orig.double_round state)
+  [SMTPat (New.chacha20_double_round state)]
   =
   ()
 
-val index_createL_lemma: #a:Type -> l:list a -> i:nat{i < List.Tot.length l} ->
-  Lemma (Seq.index 
+
+let rounds_equiv (state: New.state)
+    : Lemma (New.chacha20_rounds state == Orig.rounds state)
+  [SMTPat (New.chacha20_rounds state)]
+  =
+  fold_extensionality 10 New.chacha20_double_round Orig.double_round state
+
+let core_equiv (ctr:uint32) (state: New.state)
+    : Lemma (New.chacha20_core ctr state == Orig.chacha20_core (v ctr) state)
+  [SMTPat (New.chacha20_core ctr state)]
+  =
+    let s0 = state in
+    let s1 = array_upd state (usize 12) (
+                      (array_index (s0) (usize 12)) +. (ctr)) in
+    let k = New.chacha20_rounds s1 in
+    let ka = k `array_add (+.)` s1 in
+    let kb = k `array_add (+.)` s0 in
+    let kb' = array_upd kb (usize 12) (
+                      (array_index (kb) (usize 12)) +. (ctr)) in
+    assert (u32 (v ctr) == ctr);
+    assert(Orig.chacha20_add_counter s0 (v ctr) == s1);
+    assert(Orig.rounds s1 == New.chacha20_rounds s1);
+    assert(Orig.sum_state k s0 == kb);
+    assert(Orig.chacha20_add_counter kb (v ctr) == kb');
+    assert(ka == New.chacha20_core ctr state);
+    assert(kb' == Orig.chacha20_core (v ctr) state);
+    assert(forall i. i <> 12 ==> s0.[i] ==  s1.[i]);
+    assert(forall i. i <> 12 ==> ka.[i] ==  kb.[i]);
+    assert(forall i. i <> 12 ==> ka.[i] ==  kb'.[i]);
+    assert(s1.[12] ==  s0.[12] +. ctr);
+    assert(ka.[12] ==  k.[12] +. s1.[12]);
+    assert(kb.[12] ==  k.[12] +. s0.[12]);
+    assert(kb'.[12] ==  k.[12] +. s0.[12] +. ctr);
+    assert(kb'.[12] ==  k.[12] +. (s0.[12] +. ctr));
+    assert(kb'.[12] ==  k.[12] +. s1.[12]);
+    assert(forall i. i >= 0 /\ i < 16 ==> ka.[i] ==  kb'.[i]);
+    Lib.Sequence.eq_intro ka kb'
 
 
-let op_String_Access a b = FStar.Seq.index a b
 let constants_equiv ()
-    : Lemma (New.chacha20_constants_init () ==
-             Lib.Sequence.map secret (Orig.chacha20_constants)) =
-    let new_consts = Lib.Sequence.to_lseq (New.chacha20_constants_init ()) in
-    let old_consts = Lib.Sequence.map secret Orig.chacha20_constants in
-    assert (new_consts.[0] == secret Orig.c0);
-    assert (new_consts.[1] == secret Orig.c1);
-    assert (new_consts.[2] == secret Orig.c2);
-    assert (new_consts.[3] == secret Orig.c3);
-    assert (old_consts.[0] == secret Orig.c0);
-    assert (Seq.length new_consts == 4);
-    assert (forall i. (i > 0 /\ i < Seq.length new_consts) ==> new_consts.[i] == old_consts.[i]);
-    admit();
-    FStar.Seq.lemma_eq_intro new_consts old_consts;
-    admit()
-
-    forall (i:nat{i < 4}).
-      v (Seq.index #_ #4 (New.chacha20_constants_init ()) i) ==
-      v (Seq.index Orig.chacha20_constants i)
-    )
+    : Lemma (New.chacha20_constants_init() == Lib.Sequence.map secret Orig.chacha20_constants)
   =
   let l = [Orig.c0;Orig.c1;Orig.c2;Orig.c3] in
   assert_norm(List.Tot.length l == 4);
   assert_norm(List.Tot.index l 0 == Orig.c0);
   assert_norm(List.Tot.index l 1 == Orig.c1);
   assert_norm(List.Tot.index l 2 == Orig.c2);
-  assert_norm(List.Tot.index l 3 == Orig.c3)
+  assert_norm(List.Tot.index l 3 == Orig.c3);
+  Lib.Sequence.eq_intro (New.chacha20_constants_init ()) (Lib.Sequence.map secret Orig.chacha20_constants)
 
-let key_to_u32s_equiv (key: New.key)
-    : Lemma (New.chacha20_key_to_u32s key == Lib.ByteSequence.uints_from_bytes_le #U32 #SEC #8 key)
-  [SMTPat (New.chacha20_key_to_u32s key)]
-  =
-  let aux (i:nat{i < 8}) : Lemma (
-    Seq.index #_ #8 (New.chacha20_key_to_u32s key) i ==
-    Seq.index (Lib.ByteSequence.uints_from_bytes_le #U32 #SEC #8 key) i
-  ) =
-    Lib.ByteSequence.index_uints_from_bytes_le #U32 #SEC #8 key i
-  in
-  Classical.forall_intro aux;
-  assert(
-    New.chacha20_key_to_u32s key `Seq.equal`
-    Lib.ByteSequence.uints_from_bytes_le #U32 #SEC #8 key
-  )
+let chacha20_init_equiv (key: New.cha_cha_key) (iv:New.cha_cha_iv) (ctr:uint32)
+    : Lemma (New.chacha20_init key iv ctr ==
+             Orig.chacha20_init key iv (v ctr))
+            [SMTPat (New.chacha20_init key iv ctr)]
+  = let new_init = New.chacha20_init key iv ctr in
+    let old_init = Orig.chacha20_init key iv (v ctr) in
+    constants_equiv();
+    Lib.Sequence.eq_intro new_init old_init
 
-let iv_to_u32s_equiv (iv: New.iv)
-    : Lemma (New.chacha20_iv_to_u32s iv == Lib.ByteSequence.uints_from_bytes_le #U32 #SEC #3 iv)
-  [SMTPat (New.chacha20_iv_to_u32s iv)]
-  =
-  let aux (i:nat{i < 3}) : Lemma (
-    Seq.index #_ #3 (New.chacha20_iv_to_u32s iv) i ==
-    Seq.index (Lib.ByteSequence.uints_from_bytes_le #U32 #SEC #3 iv) i
-  ) =
-    Lib.ByteSequence.index_uints_from_bytes_le #U32 #SEC #3 iv i
-  in
-  Classical.forall_intro aux;
-  assert(
-    New.chacha20_iv_to_u32s iv `Seq.equal`
-    Lib.ByteSequence.uints_from_bytes_le #U32 #SEC #3 iv
-  )
+let chacha20_key_block_equiv (state: New.state)
+    : Lemma (New.chacha20_key_block state ==
+             Orig.chacha20_key_block state)
+            [SMTPat (New.chacha20_key_block state)] =
+            ()
 
-let ctr_to_seq_equiv (ctr: uint32)
-    : Lemma (New.chacha20_ctr_to_seq ctr == FStar.Seq.init 1 (fun _ -> ctr))
-  [SMTPat (New.chacha20_ctr_to_seq ctr)]
-  =
-  assert(New.chacha20_ctr_to_seq ctr `Seq.equal #_ #1` FStar.Seq.init 1 (fun _ -> ctr))
+let chacha20_key_block0_equiv (key: New.cha_cha_key) (iv:New.cha_cha_iv)
+    : Lemma (New.chacha20_key_block0 key iv ==
+             Orig.chacha20_key_block0 key iv)
+            [SMTPat (New.chacha20_key_block0 key iv)] =
+            ()
 
-(*
-#push-options "--z3rlimit 100"
-let chacha_block_init_equiv (key: New.key) (ctr: uint32) (iv: New.iv)
-    : Lemma (New.chacha_block_init key ctr iv ==
-      Orig.chacha20_add_counter (Orig.chacha20_init key iv 0) (v ctr))
-  = Seq.eq_intro (New.chacha_block_init key ctr iv) (Orig.chacha20_add_counter (Orig.chacha20_init key iv 0) (v ctr))
-  
-    let st = Seq.create 16 (u32 0) in
-  let st = Seq.update_sub st 0 4 (Seq.map Lib.IntTypes.secret Orig.chacha20_constants) in
-  constants_equiv ();
-  assert(Seq.sub st 0 4 `Seq.equal` New.chacha20_constants_init ());
-  let st = Seq.update_sub st 4 8 (Lib.ByteSequence.uints_from_bytes_le #U32 #SEC #8 key) in
-  assert(Seq.sub st 0 4 `Seq.equal` New.chacha20_constants_init ());
-  assert(Seq.sub st 4 8 `Seq.equal` New.chacha20_key_to_u32s key);
-  let st = Seq.(st.[12] <- u32 0) in
-  assert(Seq.sub st 0 4 `Seq.equal` New.chacha20_constants_init ());
-  assert(Seq.sub st 4 8 `Seq.equal` New.chacha20_key_to_u32s key);
-  assert(Seq.sub st 12 1 `Seq.equal` New.chacha20_ctr_to_seq (u32 0));
-  let st = Seq.update_sub st 13 3 (Lib.ByteSequence.uints_from_bytes_le #U32 #SEC #3 iv) in
-  assert(Seq.sub st 0 4 `Seq.equal` New.chacha20_constants_init ());
-  assert(Seq.sub st 4 8 `Seq.equal` New.chacha20_key_to_u32s key);
-  assert(Seq.sub st 12 1 `Seq.equal` New.chacha20_ctr_to_seq (u32 0));
-  assert(Seq.sub st 13 3 `Seq.equal` New.chacha20_iv_to_u32s iv);
-  assert(st `Seq.equal` Orig.chacha20_init key iv 0);
-  assert(New.chacha_block_init key (u32 0) iv `Seq.equal` Orig.chacha20_init key iv 0);
-  assert(Seq.(st.[12]) == u32 0);
-  let st = Seq.(st.[12] <- st.[12] +. ctr) in
-  assert(v (u32 0 +. ctr) == v ctr);
-  assert(st == Orig.chacha20_add_counter (Orig.chacha20_init key iv 0) (v ctr));
-  assert(Seq.sub st 0 4 `Seq.equal` New.chacha20_constants_init ());
-  assert(Seq.sub st 4 8 `Seq.equal` New.chacha20_key_to_u32s key);
-  assert(Seq.sub st 12 1 `Seq.equal` New.chacha20_ctr_to_seq ctr);
-  assert(Seq.sub st 13 3 `Seq.equal` New.chacha20_iv_to_u32s iv);
-  assert(st `Seq.equal` (New.chacha_block_init key ctr iv))
-#pop-options
-
-let chacha_block_inner_equiv_orig (key: New.key) (ctr: uint32) (iv: New.iv) =
-  let st0 = Orig.chacha20_init key iv 0 in
-  let st = Orig.chacha20_add_counter st0 (v ctr) in
-  let st = Orig.rounds st in
-  let st = Orig.sum_state st (Orig.chacha20_add_counter st0 (v ctr)) in
-  st
-
-let rec repeat_left (#a: Type) (n: nat) (f: a -> a) (init: a) =
-  if n = 0 then init else repeat_left (n-1) f (f init)
-
-#push-options "--fuel 1"
-let rec repeat_left_lemma (#a: Type) (n: nat) (f: a -> a) (init: a)
-  : Lemma (f (repeat_left n f init) == repeat_left n f (f init))
-  =
-  if n = 0 then () else repeat_left_lemma (n-1) f (f init)
-#pop-options
-
-#push-options "--fuel 1"
-let rec repeat_left_equals_repeat (#a: Type) (n: nat) (f: a -> a) (init: a)
-    : Lemma (Lib.LoopCombinators.repeat n f init == repeat_left n f init)
-  =
-  if n = 0 then
-    Lib.LoopCombinators.eq_repeat0 f init
-  else begin
-    Lib.LoopCombinators.unfold_repeat n f init (n-1);
-    repeat_left_equals_repeat (n-1) f (f init);
-    repeat_left_equals_repeat (n-1) f init;
-    repeat_left_lemma (n-1) f init
-  end
-#pop-options
-
-#push-options "--fuel 1"
-let rec foldi_repeat_equiv (#a: Type) (init:a) (low: uint_size) (hi: uint_size{low <= hi})
-  (f: (i:nat{i < hi}) -> a -> a)
-  (g: a -> a)
-  (equiv: (i:nat{i < hi}) -> (x:a) -> Lemma (f i x == g x))
-    : Lemma
-      (requires (True))
-      (ensures (foldi low hi f init == Lib.LoopCombinators.repeat (hi - low) g init))
-      (decreases (hi - low))
-  =
-  if low = hi then begin
-    Lib.LoopCombinators.eq_repeat0 g init;
-    assert(foldi 0 0 f init == init)
-  end else begin
-    Lib.LoopCombinators.unfold_repeat (hi - low) g init (hi - low - 1);
-    assert(Lib.LoopCombinators.repeat (hi - low) g init ==
-      g (Lib.LoopCombinators.repeat (hi - low -1) g init));
-    (* repeat is a fold_right, whereas foldi is a fold_left. Since g and f don't depend on i
-       right or left does not matter but here we should prove that repeat is equivalent to
-       repeat_left
-    *)
-    repeat_left_equals_repeat (hi - low) g init;
-    repeat_left_equals_repeat (hi - low - 1) g (g init);
-    assert(Lib.LoopCombinators.repeat (hi - low) g init ==
-      Lib.LoopCombinators.repeat (hi - low -1) g (g init));
-    foldi_repeat_equiv (g init) (low + 1) hi f g equiv;
-    equiv low init
-  end
-#pop-options
-
-let chacha_block_inner_loop1_f = fun (i_41:uint_size{i_41 < 10})  (state_40: New.state) ->
-    let state_40 = New.chacha_double_round (state_40) in
-    (state_40)
-
-let chacha_block_inner_loop1 (state_40: New.state) =
-  foldi (usize 0) (usize 10) chacha_block_inner_loop1_f
-  (state_40)
-
-let chacha_block_inner_loop1_equiv (st: New.state)
-    : Lemma (chacha_block_inner_loop1 st == Orig.rounds st)
-  =
-  foldi_repeat_equiv st 0 10
-    chacha_block_inner_loop1_f
-    Orig.double_round (fun i x -> double_round_equiv x)
-
-let chacha_block_inner_loop2_f (st_39: New.state) =
-  fun (i_42: uint_size{i_42 < 16}) (state_40: New.state) ->
-    let state_40 =
-      array_upd #_ #16 state_40 (i_42) (
-        (array_index (state_40) (i_42)) +. (array_index (st_39) (i_42)))
-    in
-    (state_40)
-
-#push-options "--fuel 2"
-let rec map2_equals_foldi_lemma1
-  (n: uint_size{n >= 1 /\ n <= 16})
-  (i: uint_size{i <= n - 1})
-  (x: New.state)
-  (y: New.state)
-    : Lemma (requires (True)) (ensures (
-      foldi i n (chacha_block_inner_loop2_f y) x ==
-      chacha_block_inner_loop2_f y (n-1) (foldi i (n-1) (chacha_block_inner_loop2_f y) x)
-    ))
-    (decreases (n - i))
-  =
-  if i = n - 1 then () else map2_equals_foldi_lemma1 n (i + 1) (chacha_block_inner_loop2_f y i x) y
-#pop-options
-
-#push-options "--fuel 2"
-let rec map2_equals_foldi_lemma2
-  (n: uint_size{n >= 1 /\ n <= 16})
-  (i: uint_size{i <= n - 1})
-  (x: New.state)
-  (y: New.state)
-    : Lemma (requires (True)) (ensures (
-      Seq.index (foldi i n (chacha_block_inner_loop2_f y) x) (n-1) ==
-      Seq.index (chacha_block_inner_loop2_f y (n-1) x) (n-1)
-    ))
-    (decreases (n - i))
-  =
-  if i = n - 1 then () else map2_equals_foldi_lemma2 n (i + 1) (chacha_block_inner_loop2_f y i x) y
-#pop-options
-
-#push-options "--fuel 2 --z3rlimit 30"
-let rec map2_equals_foldi
-  (n: uint_size{n >= 1 /\ n <= 16})
-  (x: New.state)
-  (y: New.state)
-    : Lemma (Seq.sub (Seq.map2 (+.) x y) 0 n ==
-      Seq.sub (foldi 0 n (chacha_block_inner_loop2_f y) x) 0 n)
-  =
-  if n = 1 then begin
-    assert(Seq.sub (Seq.map2 (+.) x y) 0 n `Seq.equal`
-      Seq.sub (foldi 0 n (chacha_block_inner_loop2_f y) x) 0 n)
-  end else begin
-    map2_equals_foldi (n-1) x y;
-    assert(Seq.sub (Seq.map2 (+.) x y) 0 (n-1) `Seq.equal`
-
-      Seq.sub (foldi 0 (n-1) (chacha_block_inner_loop2_f y) x) 0 (n-1));
-    let aux (i: nat{i < n}) : Lemma (Seq.index (Seq.sub (Seq.map2 (+.) x y) 0 n) i ==
-      Seq.index (Seq.sub (foldi 0 n (chacha_block_inner_loop2_f y) x) 0 n) i)
-      =
-      if i < n-1 then begin
-        assert(Seq.index (Seq.sub (Seq.map2 (+.) x y) 0 n) i ==
-          Seq.index (Seq.sub (Seq.map2 (+.) x y) 0 (n-1)) i);
-        map2_equals_foldi_lemma1 n 0 x y;
-        assert(Seq.index (foldi 0 (n-1) (chacha_block_inner_loop2_f y) x) i ==
-          Seq.index (foldi 0 n (chacha_block_inner_loop2_f y) x) i)
-      end else begin
-        assert(Seq.index (Seq.sub (foldi 0 n (chacha_block_inner_loop2_f y) x) 0 n) i ==
-          Seq.index (foldi 0 n (chacha_block_inner_loop2_f y) x) (n-1));
-        map2_equals_foldi_lemma2 n 0 x y
-      end
-    in
-    Classical.forall_intro aux;
-    assert(Seq.sub (Seq.map2 (+.) x y) 0 n `Seq.equal`
-      Seq.sub (foldi 0 n (chacha_block_inner_loop2_f y) x) 0 n)
-  end
-#pop-options
-
-let chacha_block_inner_loop2 (state_40: New.state) (st_39: New.state) =
-  foldi (usize 0) (usize 16) (chacha_block_inner_loop2_f st_39) (state_40)
-
-let chacha_block_inner_loop2_equiv (st st0: New.state)
-    : Lemma (chacha_block_inner_loop2 st st0 == Orig.sum_state st st0)
-  =
-  map2_equals_foldi 16 st st0
-
-let chacha_block_inner_alt (key: New.key) (ctr: uint32) (iv: New.iv) =
-  let st = New.chacha_block_init key ctr iv in
-  let st0 = st in
-  let st = chacha_block_inner_loop1 st in
-  let st = chacha_block_inner_loop2 st st0 in
-  st
-
-open FStar.Tactics
-
-let chacha_block_inner_new_comp (key: New.key) (ctr: uint32) (iv: New.iv)
-  : Lemma (New.chacha_block_inner key ctr iv == chacha_block_inner_alt key ctr iv)
-  =
-  assert(New.chacha_block_inner key ctr iv == chacha_block_inner_alt key ctr iv) by begin
-    norm [delta_only [
-      "Hacspec.Chacha20.chacha_block_inner";
-      "Hacspec.Chacha20.Proof.chacha_block_inner_alt";
-      "Hacspec.Chacha20.Proof.chacha_block_inner_loop1";
-      "Hacspec.Chacha20.Proof.chacha_block_inner_loop1_f";
-      "Hacspec.Chacha20.Proof.chacha_block_inner_loop2";
-      "Hacspec.Chacha20.Proof.chacha_block_inner_loop2_f";
-      "Hacspec.Chacha20.state"
-    ]];
-    smt ()
-  end
-
-let chacha_block_inner_equiv_orig2 (key: New.key) (ctr: uint32) (iv: New.iv) =
-  let st0 = Orig.chacha20_init key iv 0 in
-  let st = Orig.chacha20_core (v ctr) st0 in
-  st
-
-#push-options "--z3rlimit 50"
-let sum_assoc (x y z: uint32) : Lemma (x +. y +. z == x +. (y +. z)) =
-  assert(v (x +. y +. z) = (v x + v y + v z) % modulus U32);
-  assert(v (y +. z) = (v y + v z) % modulus U32);
-  assert(v (x +. (y +. z)) = (v x + ((v y + v z) % modulus U32)) % modulus U32);
-  FStar.Math.Lemmas.lemma_mod_mod (v (x +. (y +. z))) (v x + ((v y + v z) )) (modulus U32);
-  assert(v (x +. (y +. z)) = (v x + v y + v z) % modulus U32)
-#pop-options
-
-#push-options "--z3rlimit 15"
-let sum_state_and_add_counter_commute (x: New.state) (y: New.state) (c: uint32)
-  : Lemma (Orig.sum_state x (Orig.chacha20_add_counter y (v c)) ==
-          Orig.chacha20_add_counter (Orig.sum_state x y) (v c))
-  =
-  let aux (i:nat{i < 16}) : Lemma (
-    Seq.index (Orig.sum_state x (Orig.chacha20_add_counter y (v c))) i ==
-          Seq.index (Orig.chacha20_add_counter (Orig.sum_state x y) (v c)) i
-  ) =
-    assert(Seq.index (Orig.sum_state x (Orig.chacha20_add_counter y (v c))) i ==
-      Seq.index x i +. Seq.index (Orig.chacha20_add_counter y (v c)) i);
-    if i = 12 then begin
-      assert(Seq.index (Orig.chacha20_add_counter y (v c)) i == Seq.index y i +. c);
-      assert(Seq.index (Orig.chacha20_add_counter (Orig.sum_state x y) (v c)) i ==
-        Seq.index (Orig.sum_state x y) i +. c);
-      assert(Seq.index (Orig.sum_state x y) i +. c ==
-        Seq.index x i +. Seq.index y i +. c);
-      assert(Seq.index x i +. Seq.index (Orig.chacha20_add_counter y (v c)) i ==
-        Seq.index x i +. (Seq.index y i +. c));
-      sum_assoc (Seq.index x i) (Seq.index y i) c;
-      assert(Seq.index x i +. Seq.index y i +. c == Seq.index x i +. (Seq.index y i +. c))
-    end else begin
-      assert(Seq.index (Orig.chacha20_add_counter y (v c)) i == Seq.index y i);
-      assert(Seq.index (Orig.chacha20_add_counter (Orig.sum_state x y) (v c)) i ==
-        Seq.index (Orig.sum_state x y) i)
-    end
-  in
-  Classical.forall_intro aux;
-  assert(Orig.sum_state x (Orig.chacha20_add_counter y (v c)) `Seq.equal`
-          Orig.chacha20_add_counter (Orig.sum_state x y) (v c))
-#pop-options
-
-let chacha_block_inner_equiv_orig_1_2_equiv (key: New.key) (ctr: uint32) (iv: New.iv)
-    : Lemma (chacha_block_inner_equiv_orig key ctr iv == chacha_block_inner_equiv_orig2 key ctr iv)
-  =
-  let st0 = Orig.chacha20_init key iv 0 in
-  let st_1 = Orig.chacha20_add_counter st0 (v ctr) in
-  let st_2 = Orig.chacha20_add_counter st0 (v ctr) in
-  let st_1 = Orig.rounds st_1 in
-  let st_2 = Orig.rounds st_2 in
-  assert(st_1 == st_2);
-  sum_state_and_add_counter_commute st_1 st0 ctr;
-  let st_1 = Orig.sum_state st_1 (Orig.chacha20_add_counter st0 (v ctr)) in
-  let st_2 = Orig.sum_state st_2 st0 in
-  let st_2 = Orig.chacha20_add_counter st_2 (v ctr) in
-  assert(st_1 == chacha_block_inner_equiv_orig key ctr iv);
-  assert(st_2 == chacha_block_inner_equiv_orig2 key ctr iv)
-
-let chacha_block_inner_equiv (key: New.key) (ctr: uint32) (iv: New.iv)
-    : Lemma (chacha_block_inner_alt key ctr iv == chacha_block_inner_equiv_orig key ctr iv)
-  =
-  let st0' = Orig.chacha20_init key iv 0 in
-  let st' = Orig.chacha20_add_counter st0' (v ctr) in
-  let st = New.chacha_block_init key ctr iv in
-  let st0 = st in
-  chacha_block_init_equiv key ctr iv;
-  assert(st0 == st');
-  chacha_block_inner_loop1_equiv st;
-  let st' = Orig.rounds st' in
-  let st = chacha_block_inner_loop1 st in
-  chacha_block_inner_loop2_equiv st st0;
-  let st' = Orig.sum_state st' (Orig.chacha20_add_counter st0' (v ctr)) in
-  let st = chacha_block_inner_loop2 st st0 in
-  assert(st' == chacha_block_inner_equiv_orig key ctr iv);
-  assert(st == chacha_block_inner_alt key ctr iv)
-
-let state_to_bytes_loop
-  (x_0: New.state)
-  (i_2:nat{i_2 <16})
-  (r_1: New.state_bytes)
-    : New.state_bytes
-  =
-  let bytes_3 = uint32_to_be_bytes (array_index (x_0) (i_2)) in
-  let r_1 =
-    array_upd r_1 ((i_2) * (usize 4)) (array_index (bytes_3) (usize 3))
-  in
-  let r_1 =
-    array_upd r_1 (((i_2) * (usize 4)) + (usize 1)) (
-      array_index (bytes_3) (usize 2))
-  in
-  let r_1 =
-    array_upd r_1 (((i_2) * (usize 4)) + (usize 2)) (
-      array_index (bytes_3) (usize 1))
-  in
-  let r_1 =
-    array_upd r_1 (((i_2) * (usize 4)) + (usize 3)) (
-      array_index (bytes_3) (usize 0))
-  in
-  (r_1)
-
-let state_to_bytes_equiv_aux (st: New.state) : Lemma (New.state_to_bytes st == (
-  let r = array_new_ (u8 0x8) 64 in
-  foldi 0 16 (state_to_bytes_loop st) r)
-)
-  =
-  assert(New.state_to_bytes st == (
-  let r = array_new_ (secret (pub_u8 0x8)) 64 in
-  let open FStar.Tactics in
-  foldi (usize 0) (array_len st) (state_to_bytes_loop st) r)) by begin
-    norm [delta_only [
-      "Hacspec.Chacha20.state_to_bytes";
-      "Hacspec.Chacha20.Proof.state_to_bytes_loop"
-    ]];
-    compute ()
-  end
-
-let state_to_bytes_loop_equiv (x: New.state) (i:nat{i < 16}) (r: New.state_bytes)
-    : Lemma (Seq.sub (state_to_bytes_loop x i r) (4 * i) 4 ==
-      Lib.ByteSequence.uint_to_bytes_le (Seq.index x i)
-    )
-  =
-  Lib.ByteSequence.index_uint_to_bytes_le (Seq.index x i);
-  assume(Seq.sub (state_to_bytes_loop x i r) (4 * i) 4 `Seq.equal`
-    Lib.ByteSequence.uint_to_bytes_le (Seq.index x i))
-
-let state_to_bytes_equiv (st: New.state)
-    : Lemma (
-      New.state_to_bytes st == Lib.ByteSequence.uints_to_bytes_le st)
-  =
-  Classical.forall_intro (Lib.ByteSequence.index_uints_to_bytes_le st);
-  assume(New.state_to_bytes st `Seq.equal` Lib.ByteSequence.uints_to_bytes_le st)
-
-unfold let chacha20_main_loop_inner
-  (key_47: New.key) (iv_48: New.iv)
-  (i_52:uint_size)
-  (block_len_53: uint_size{block_len_53 <= 64})
-  (msg_block_54: lseq uint8 block_len_53)
-  (ctr_50:uint32)
-  =
-  let key_block_55 = New.chacha_block (key_47) (ctr_50) (iv_48) in
-  let msg_block_padded_56 = array_new_ (secret (pub_u8 0x8)) (64) in
-  let msg_block_padded_57 =
-    array_update_start (msg_block_padded_56) (msg_block_54)
-  in
-  array_slice_range (
-   (msg_block_padded_57) `array_xor (^.)` (key_block_55)) (
-     (usize 0, block_len_53))
-
-let chacha20_main_loop_alt (key_47: New.key) (iv_48: New.iv) (m_49: byte_seq)
-  (i_52:uint_size{i_52 < seq_num_chunks (m_49) (usize 64)})
-  (tup: (uint32 & lseq uint8 (seq_len m_49)))
-    : (uint32 & lseq uint8 (seq_len m_49))
-  =
-  let (ctr_50, blocks_out_51) = tup in
-  let (block_len_53, msg_block_54) =
-    seq_get_chunk (m_49) (usize 64) (i_52)
-  in
-  let blocks_out_51 =
-    seq_set_chunk (blocks_out_51) (usize 64) (i_52) (
-      chacha20_main_loop_inner key_47 iv_48 i_52 block_len_53 msg_block_54 ctr_50)
-  in
-  let ctr_50 = (ctr_50) +. (secret (pub_u32 0x1)) in
-  (ctr_50, blocks_out_51)
-
-let chacha20_main_loop (key_47: New.key) (iv_48: New.iv) (m_49: byte_seq)
-  (i_52:uint_size{i_52 < seq_num_chunks (m_49) (usize 64)})
-  (tup: (uint32 & lseq uint8 (seq_len m_49)))
-    : (uint32 & lseq uint8 (seq_len m_49))
-  =
-  let (ctr_50, blocks_out_51) = tup in
-  let (block_len_53, msg_block_54) =
-    seq_get_chunk (m_49) (usize 64) (i_52)
-  in
-   let key_block_55 = New.chacha_block (key_47) (ctr_50) (iv_48) in
-  let msg_block_padded_56 = array_new_ (secret (pub_u8 0x8)) (64) in
-  let msg_block_padded_57 =
-    array_update_start (msg_block_padded_56) (msg_block_54)
-  in
-  let blocks_out_51 =
-    seq_set_chunk (blocks_out_51) (usize 64) (i_52) ( array_slice_range (
-   (msg_block_padded_57) `array_xor (^.)` (key_block_55)) (
-     (usize 0, block_len_53)))
-  in
-  let ctr_50 = (ctr_50) +. (secret (pub_u32 0x1)) in
-  (ctr_50, blocks_out_51)
-
-let chacha20_main_loop_equiv (key_47: New.key) (iv_48: New.iv) (m_49: byte_seq)
-  (i_52:uint_size{i_52 < seq_num_chunks (m_49) (usize 64)})
-  (tup: (uint32 & lseq uint8 (seq_len m_49)))
-    : Lemma (chacha20_main_loop key_47 iv_48 m_49 i_52 tup ==
-      chacha20_main_loop_alt key_47 iv_48 m_49 i_52 tup)
-  =
-  ()
-
-let chacha20_alt_alt (key: New.key) (iv: New.iv) (m: byte_seq) =
-  let ctr = secret (pub_u32 0x1) in
-  let blocks_out = seq_new_ (secret (pub_u8 0x8)) (seq_len m) in
-  let ctr, blocks_out = foldi (usize 0) (seq_num_chunks m (usize 64))
-    (chacha20_main_loop_alt key iv m) (ctr, blocks_out)
-  in
-  blocks_out
-
-let chacha20_alt (key: New.key) (iv: New.iv) (m: byte_seq) =
-  let ctr = secret (pub_u32 0x1) in
-  let blocks_out = seq_new_ (secret (pub_u8 0x8)) (seq_len m) in
-  let ctr, blocks_out = foldi (usize 0) (seq_num_chunks m (usize 64))
-    (chacha20_main_loop key iv m) (ctr, blocks_out)
-  in
-  blocks_out
-
-let chacha20_alt_alt_equiv (key: New.key) (iv: New.iv) (m: byte_seq)
-    : Lemma (chacha20_alt key iv m == chacha20_alt_alt key iv m)
-  =
-  // Need another foldi lemma using chacha20_main_loop_equiv...
-  admit()
-
-let chacha20_equiv_one_iter
-  (key: New.key)
-  (iv: New.iv)
-  (i:uint_size{i + 1 < maxint U32})
-  (x: lseq uint8 64)
-    : Lemma(Orig.chacha20_encrypt_block (Orig.chacha20_init key iv 0) i x ==
-      chacha20_main_loop_inner key iv i 64 x (u32 (i + 1)))
-  =
-  // To prove using chacha_block_inner_alt_equiv and stuff like this
-  admit()
+let chacha20_encrypt_block_equiv (state: New.state) (ctr:uint32) (plain:New.block)
+    : Lemma (New.chacha20_encrypt_block state ctr plain ==
+             Orig.chacha20_encrypt_block state (v ctr) plain)
+            [SMTPat (New.chacha20_encrypt_block state ctr plain)] =
+            ()
 
 
-let chacha20_equiv_aux1 (key: New.key) (iv: New.iv) (m: byte_seq)
-    : Lemma (chacha20_alt_alt key iv m == Orig.chacha20_decrypt_bytes key iv 0 m)
-  =
-  let st0 = Orig.chacha20_init key iv 0 in
-  let st =  Lib.Sequence.map_blocks 64 m
-    (Orig.chacha20_encrypt_block st0)
-    (Orig.chacha20_encrypt_last st0) in
+let chacha20_encrypt_last_equiv (state: New.state) (ctr:uint32) (plain:byte_seq{seq_len plain < 64})
+    : Lemma (New.chacha20_encrypt_last state ctr plain ==
+             Orig.chacha20_encrypt_last state (v ctr) (seq_len plain) plain)
+            [SMTPat (New.chacha20_encrypt_last state ctr plain)] =
+    let orig_last = Orig.chacha20_encrypt_last state (v ctr) (seq_len plain) plain in
+    let new_last = New.chacha20_encrypt_last state ctr plain in
+    Lib.Sequence.eq_intro orig_last new_last
 
-  let ctr = secret (pub_u32 0x1) in
-  let blocks_out = seq_new_ (secret (pub_u8 0x8)) (seq_len m) in
-  let ctr, blocks_out = foldi (usize 0) (seq_num_chunks m (usize 64))
-    (chacha20_main_loop_alt key iv m) (ctr, blocks_out)
-  in
-  // Use chacha20_equiv_one_iter and chacha20_equiv_one_iter_last
-  assume(blocks_out == st)
 
-let chacha20_alt_equiv (key: New.key) (iv: New.iv) (m: byte_seq)
-  : Lemma (chacha20_alt key iv m == New.chacha key iv m)
-  =
-  let open FStar.Tactics in
-  assert(chacha20_alt key iv m == New.chacha key iv m) by begin
-    norm [delta_only [
-      "Hacspec.Chacha20.Proof.chacha20_alt";
-      "Hacspec.Chacha20.Proof.chacha20_main_loop";
-      "Hacspec.Chacha20.chacha"
-    ]];
-    smt ()
-  end
+let chacha20_update_equiv (state: New.state) (m:byte_seq)
+    : Lemma (New.chacha20_update state m ==
+             Orig.chacha20_update state m)
+            [SMTPat (New.chacha20_update state m)] = admit()
 
-(* This is the main theorem *)
-let chacha20_equiv (key: New.key) (iv: New.iv) (m: byte_seq)
-    : Lemma (New.chacha key iv m == Orig.chacha20_encrypt_bytes key iv 0 m)
-  =
-  chacha20_equiv_aux1 key iv m;
-  chacha20_alt_alt_equiv key iv m;
-  chacha20_alt_equiv key iv m
+
+let chacha20_equiv (key : New.cha_cha_key) (iv : New.cha_cha_iv) (ctr : pub_uint32) (m : byte_seq)
+  : Lemma (New.chacha20 key iv ctr m ==
+           Orig.chacha20_encrypt_bytes key iv (v ctr) m) = ()
